iris/AppTree.v
@@ -154,6 +154,8 @@ Require Import TreeView.         (* TL-1: [subtree], [own_wf], the deltas *)
 Require Import AppInv.           (* [app_sup_raw], [app_xfer_raw] *)
 Require ConsLog.               (* [cons_step] / [cons_ev]: the merged console claim's event type *)
 Require Import SystemAdequacy.   (* [app_xfer_boot_raw]: [App.Happ_boot] *)
+Require Import RiscvPtsto.       (* [app_iface_triv]: the interface a
+                                    tree application sets *)
 Require Import App.              (* [xv6_app], [MkApp] *)
 
 Local Open Scope Z_scope.
@@ -1154,12 +1156,11 @@ Section AppTreeRecord.
     MkApp tree_fixed tree_cl tree_names tree_pred
           tree_boot                          (* app_boot *)
           tree_R                             (* app_R *)
-          (fun _ _ => True%I)                (* app_tag *)
-          (fun _ => True%I)                  (* app_kill *)
+          (* THE CONSOLE INTERFACE (upstream redesign R2/R4): a tree
+             application says nothing about a received byte, puts no price
+             on a kill and claims nothing of the console *)
+          (fun _ => app_iface_triv Σ)        (* app_ifc *)
           (fun _ _ => emp%I)                 (* app_turn *)
-          (* the console claim (upstream redesign R2/R3): a tree
-             application claims nothing of the console *)
-          (fun _ _ _ _ => emp%I)             (* app_cons *)
           (fun _ _ => True).                 (* app_phi *)
 
   (* ---- the obligations of [App.xv6_app_adequacy] that are lemmas ---- *)
@@ -1188,7 +1189,10 @@ Section AppTreeRecord.
   (* A KILL COSTS THIS APPLICATION NOTHING (design section 3) *)
   Lemma app_tree_kill (c : app_fixed app_tree) (r : app_names app_tree) :
     app_sup_raw (app_pred app_tree c) r ⊢ □ app_kill app_tree c.
-  Proof. cbn [app_tree app_kill]. iIntros "_ !>". done. Qed.
+  Proof.
+    rewrite /app_kill. cbn [app_tree app_ifc app_iface_triv ai_kill].
+    iIntros "_ !>". done.
+  Qed.
 
   (* ONE LICENCE over the console claim (redesign R2): the tree
      application's claim is [emp], so every console event on it is free;
@@ -1199,11 +1203,10 @@ Section AppTreeRecord.
              (ev : ConsLog.cons_ev),
              app_cons app_tree c k h H ==∗
              app_cons app_tree c k h (ConsLog.cons_step H ev)).
-  Proof. cbn [app_tree app_cons]. iIntros "_ !>" (k h H ev) "_". by iModIntro. Qed.
-
-  Lemma app_tree_const (c : app_fixed app_tree) (k : nat) (h : list mobs)
-      (H : LogEntryDefs.cons_hist) : Timeless (app_cons app_tree c k h H).
-  Proof. cbn [app_tree app_cons]. apply _. Qed.
+  Proof.
+    rewrite /app_cons. cbn [app_tree app_ifc app_iface_triv ai_cons].
+    rewrite /cons_res_triv. iIntros "_ !>" (k h H ev) "_". by iModIntro.
+  Qed.
 
   Lemma app_tree_R0 (c : app_fixed app_tree) :
     app_cl app_tree c ⊢ |==> app_R app_tree c [].
@@ -1224,7 +1227,8 @@ Section AppTreeRecord.
               (LogEntryDefs.MkCH [] [] [] None) ∗
             app_turn app_tree c (S (obs_boots h))).
   Proof.
-    intros _. cbn [app_tree app_R app_cons app_turn].
+    intros _. rewrite /app_cons.
+    cbn [app_tree app_R app_ifc app_iface_triv ai_cons app_turn].
     iIntros "H". iModIntro. iSplitL "H"; [iExact "H" |].
     destruct on; by repeat iSplitR.
   Qed.
@@ -1242,8 +1246,7 @@ End AppTreeRecord.
 (*  7.  WHAT THE RECORD STILL OWES ([App.xv6_app_adequacy]'s binders)     *)
 (*                                                                       *)
 (*  Discharged above, as lemmas at the record's fields: [Hbirth], [HRt],  *)
-(*  [Htagp], [Htagt], [Hkillp], [Hkillt], [Happ_kill], [Hconst],          *)
-(*  [Happ_out_sup], [HR0], [Hpow], [Happ_boot].                            *)
+(*  [Happ_kill], [Happ_out_sup], [HR0], [Hpow], [Happ_boot].               *)
 (*                                                                       *)
 (*  Trivial at this record's fields and left to the instance site (they   *)
 (*  are [app_triv]'s one-liners at [emp] claims -- see                    *)
